Added interface and documentation

ulib/experimental/Steel.PCM.ArrayStruct.fst
@@ -24,61 +24,7 @@ open Steel.PCM
 open Steel.PCM.Unitless
 module SizeT = Steel.SizeT
 
-
-
 #set-options "--fuel 1 --ifuel 1"
-
-type field_id = string
-
-/// The descriptor contains all the information necessary to derive the type of the values
-/// corresponding to an arraystruct.
-noeq
-type array_struct_descriptor : Type u#(a + 1) =
-  | DBase : a: Type u#a -> array_struct_descriptor
-  | DArray : cell_descriptor: array_struct_descriptor u#a -> len: SizeT.t -> array_struct_descriptor
-  | DStruct : field_descriptors: (field_id ^-> array_struct_descriptor u#a)
-    -> array_struct_descriptor
-
-// Missing: untagged unions (not must have)
-unfold
-let struct_field_type'
-      (field_descriptors: (field_id ^-> array_struct_descriptor u#a))
-      (array_struct_type:
-          (descriptor: array_struct_descriptor u#a {descriptor << field_descriptors}
-              -> Tot (Type u#a)))
-      (field: field_id)
-    : Tot (Type u#a) =
-  let descr = field_descriptors field in
-  FStar.WellFounded.axiom1 field_descriptors field;
-  array_struct_type descr
-
-let array_type (cell_type: Type u#a) (len: SizeT.t) : Type u#a = Seq.lseq cell_type (SizeT.v len)
-
-let struct_type (field_typs: (field_id -> Type u#a)) : Type u#a = DepMap.t field_id field_typs
-
-/// This functions achives the descriptor -> Type correspondence
-let rec array_struct_type (descriptor: array_struct_descriptor u#a)
-    : Tot (Type u#a) (decreases descriptor) =
-  match descriptor with
-  | DBase a -> a
-  | DArray descriptor' len ->
-    let typ' = array_struct_type descriptor' in
-    array_type typ' len
-  | DStruct field_descriptors ->
-    let typs' = struct_field_type' field_descriptors array_struct_type in
-    struct_type typs'
-unfold
-let struct_field_type
-      (field_descriptors: (field_id ^-> (array_struct_descriptor u#a)))
-      (field: field_id)
-    : Tot (Type u#a) = struct_field_type' field_descriptors array_struct_type field
-noeq
-type array_struct : Type u#(a + 1) =
-  | ArrayStruct :
-      descriptor: array_struct_descriptor u#a ->
-      pcm: unitless_pcm (array_struct_type descriptor) ->
-      value: array_struct_type descriptor
-    -> array_struct
 
 let struct_field_type_unroll_lemma (field_descriptors: (field_id ^-> array_struct_descriptor u#a))
     : Lemma
@@ -88,63 +34,12 @@ let struct_field_type_unroll_lemma (field_descriptors: (field_id ^-> array_struc
   FStar.Tactics.Effect.assert_by_tactic (DependentMap.t field_id
         (struct_field_type field_descriptors) ==
       array_struct_type (DStruct field_descriptors))
-    (fun _ ->
-        ();
-        compute ())
-
-/// Composability is then based on the composability of the nested PCM.
-let composable_array_struct:symrel u#(a + 1) (array_struct u#a) =
-  fun (s0: array_struct u#a) (s1: array_struct u#a) ->
-    s0.descriptor == s1.descriptor /\ s0.pcm == s1.pcm /\
-    s0.pcm.unitless_p.unitless_composable s0.value s1.value
-
-let compose_array_struct
-      (s0: array_struct u#a)
-      (s1: array_struct u#a {s0 `composable_array_struct` s1})
-    : array_struct u#a =
-  let new_val = s0.pcm.unitless_p.unitless_op s0.value s1.value in
-  ArrayStruct s0.descriptor s0.pcm new_val
-
-#set-options "--print_universes --print_implicits"
-
-let array_struct_unitless_pcm':unitless_pcm' u#(a + 1) (array_struct u#a) =
-  { unitless_composable = composable_array_struct u#a; unitless_op = compose_array_struct u#a }
-
-let array_struct_unitless_pcm:unitless_pcm u#(a + 1) (array_struct u#a) =
-  {
-    unitless_p = array_struct_unitless_pcm' u#a;
-    unitless_comm = (fun s0 s1 -> s0.pcm.unitless_comm s0.value s1.value);
-    unitless_assoc = (fun s0 s1 s2 -> s0.pcm.unitless_assoc s0.value s1.value s2.value);
-    unitless_assoc_r = (fun s0 s1 s2 -> s0.pcm.unitless_assoc_r s0.value s1.value s2.value)
-  }
-
-let array_struct_pcm:pcm u#(a + 1) (option u#(a + 1) (array_struct u#a)) =
-  to_full_pcm_with_unit array_struct_unitless_pcm
-
-////////////////////////////////////////////////////////////////////
-// PCM builders
-////////////////////////////////////////////////////////////////////
+    (fun _ -> compute ())
 
 let pointwise_array_pcm (cell_type: Type u#a) (len: SizeT.t) (base_pcm: unitless_pcm cell_type)
     : unitless_pcm (array_type cell_type len) =
-  let composable_cell (x y: array_type cell_type len) (i: nat{i < SizeT.v len}) : prop =
-    let xi = Seq.index x i in
-    let yi = Seq.index y i in
-    base_pcm.unitless_p.unitless_composable xi yi
-  in
-  let composable:symrel (array_type cell_type len) =
-    fun x y -> forall (i: nat{i < SizeT.v len}). composable_cell x y i
-  in
-  let compose (x: array_type cell_type len) (y: array_type cell_type len {composable x y})
-      : array_type cell_type len =
-    Seq.init (SizeT.v len)
-      (fun i ->
-          let xi = Seq.index x i in
-          let yi = Seq.index y i in
-          base_pcm.unitless_p.unitless_op xi yi)
-  in
   let pcm':unitless_pcm' (array_type cell_type len) =
-    { unitless_composable = composable; unitless_op = compose }
+    { unitless_composable = composable_array base_pcm; unitless_op = compose_array base_pcm }
   in
   {
     unitless_p = pcm';
@@ -202,27 +97,21 @@ let pointwise_array_pcm (cell_type: Type u#a) (len: SizeT.t) (base_pcm: unitless
         assert (x_yz `Seq.equal` xy_z))
   }
 
+let reveal_pointwise_array_pcm
+      (cell_type: Type u#a)
+      (len: SizeT.t)
+      (base_pcm: unitless_pcm cell_type)
+    : Lemma
+    (let pcm = pointwise_array_pcm cell_type len base_pcm in
+      pcm.unitless_p.unitless_composable == composable_array base_pcm /\
+      pcm.unitless_p.unitless_op == compose_array base_pcm) = ()
+
 let pointwise_struct_pcm
       (field_types: (field_id -> Type u#a))
       (base_pcms: (field: field_id -> unitless_pcm (field_types field)))
     : unitless_pcm (struct_type field_types) =
-  let composable_field (field: field_id) (x y: struct_type field_types) : prop =
-    let xf = DepMap.sel x field in
-    let yf = DepMap.sel y field in
-    (base_pcms field).unitless_p.unitless_composable xf yf
-  in
-  let composable:symrel (struct_type field_types) =
-    fun x y -> forall (field: field_id). composable_field field x y
-  in
-  let compose (x: struct_type field_types) (y: struct_type field_types {composable x y})
-      : struct_type field_types =
-    DepMap.create (fun field ->
-          let xf = DepMap.sel x field in
-          let yf = DepMap.sel y field in
-          (base_pcms field).unitless_p.unitless_op xf yf)
-  in
   let pcm':unitless_pcm' (struct_type field_types) =
-    { unitless_composable = composable; unitless_op = compose }
+    { unitless_composable = composable_struct base_pcms; unitless_op = compose_struct base_pcms }
   in
   {
     unitless_p = pcm';
@@ -285,57 +174,11 @@ let pointwise_struct_pcm
         assert (x_yz `DepMap.equal` xy_z))
   }
 
-////////////////////////////////////////////////////////////////////
-// Examples
-////////////////////////////////////////////////////////////////////
+let reveal_pointwise_struct_pcm
+      (field_types: (field_id -> Type u#a))
+      (base_pcms: (field: field_id -> unitless_pcm (field_types field)))
+    : Lemma
+    (let pcm = pointwise_struct_pcm field_types base_pcms in
+      pcm.unitless_p.unitless_composable == composable_struct base_pcms /\
+      pcm.unitless_p.unitless_op == compose_struct base_pcms) = ()
 
-open Steel.PCM.FractionalPermission
-open Steel.PCM.Unitless.Base
-
-let array_with_frac_perm_on_all_indexes (t: Type u#a) (len: SizeT.t) (v: t) : array_struct u#a =
-  ArrayStruct (DArray (DBase (with_perm u#a t)) len)
-    (pointwise_array_pcm (with_perm t) len frac_perm_pcm)
-    (Seq.init u#a (SizeT.v len) (fun _ -> { value = v; perm = perm_one }))
-
-let immutable_splittable_array (t: Type u#a) (len: SizeT.t) (v: t) : array_struct u#a =
-  ArrayStruct (DArray (DBase t) len)
-    (pointwise_array_pcm t len immutable_unitless_pcm)
-    (Seq.init u#a (SizeT.v len) (fun _ -> v))
-
-let two_fields_restricted_func
-      (#a: Type u#a)
-      (field1: string)
-      (field2: string{field2 <> field1})
-      (value1 value2 by_default: a)
-    : (field_id ^-> a) =
-  on _
-    (fun field -> if field = field1 then value1 else if field = field2 then value2 else by_default)
-
-#push-options "--fuel 2 --ifuel 2"
-let two_fields_dep_map
-      (a: (field_id -> Type u#a))
-      (field1: string)
-      (field2: string{field2 <> field1})
-      (value1: a field1)
-      (value2: a field2)
-      (by_default: (field: field_id{field <> field1 /\ field <> field2} -> a field))
-    : (DepMap.t field_id a) =
-  DepMap.create #field_id
-    #a
-    (fun field ->
-        if field = field1 then value1 else if field = field2 then value2 else by_default field)
-
-
-let point_2d:array_struct =
-  let field_descriptors = two_fields_restricted_func "x" "y" (DBase int) (DBase int) (DBase unit) in
-  let field_types:(field_id -> Type0) = struct_field_type field_descriptors in
-  let field_pcms:(field: field_id -> unitless_pcm (field_types field)) =
-    fun field ->
-      if field = "x"
-      then exclusive_unitless_pcm
-      else if field = "y" then immutable_unitless_pcm else exclusive_unitless_pcm
-  in
-  struct_field_type_unroll_lemma field_descriptors;
-  ArrayStruct (DStruct field_descriptors)
-    (pointwise_struct_pcm field_types field_pcms)
-    (two_fields_dep_map field_types "x" "y" 0 1 (fun _ -> ()))
