ulib/experimental/Steel.PCM.ArrayStruct.fsti
@@ -1,0 +1,315 @@
+(*
+   Copyright 2020 Microsoft Research
+
+   Licensed under the Apache License, Version 2.0 (the "License");
+   you may not use this file except in compliance with the License.
+   You may obtain a copy of the License at
+
+       http://www.apache.org/licenses/LICENSE-2.0
+
+   Unless required by applicable law or agreed to in writing, software
+   distributed under the License is distributed on an "AS IS" BASIS,
+   WITHOUT WARRANTIES OR CONDITIONS OF ANY KIND, either express or implied.
+   See the License for the specific language governing permissions and
+   limitations under the License.
+*)
+
+module Steel.PCM.ArrayStruct
+
+module SizeT = Steel.SizeT
+module DepMap = FStar.DependentMap
+
+open FStar.FunctionalExtensionality
+open Steel.PCM
+open Steel.PCM.Unitless
+
+/// The C language allows the definition of flat data structure composed of nested struts and arrays.
+/// These flat data structures are used everywhere in systems programming, as their size can be
+/// computed at compile time and they can be statically or stack-allocated. In the following, we will
+/// refer to these data structures as arraystructs.
+///
+/// This module defines the memory-model-compatible representation of arraystructs:
+/// - the `arraystruct` type that will be stored inside memory references
+/// - helper functions to build partial commutative monoids for arraystructs
+/// - examples of use
+
+(*** The [arraystruct] type *)
+
+(**** Descriptors *)
+
+/// Since an arraystruct can contain multiple levels of nested arrays and struct, we need to be able
+/// to describe precisely the nesting structure. That is what a descriptor achieves.
+
+(** The field of structs are designated by a string (the name of the field) *)
+type field_id = string
+
+(**
+  The descriptor contains all the information necessary to derive the type of the values
+  corresponding to an arraystruct.
+*)
+noeq
+type array_struct_descriptor : Type u#(a + 1) =
+  | DBase : a: Type u#a -> array_struct_descriptor
+  | DArray : cell_descriptor: array_struct_descriptor u#a -> len: SizeT.t -> array_struct_descriptor
+  | DStruct : field_descriptors: (field_id ^-> array_struct_descriptor u#a)
+    -> array_struct_descriptor
+
+(**** [arraystruct] values type *)
+
+(** The type of an array value is an [lseq] *)
+let array_type (cell_type: Type u#a) (len: SizeT.t) : Type u#a = Seq.lseq cell_type (SizeT.v len)
+
+(** The type of a struct type is a dependent map *)
+let struct_type (field_typs: (field_id -> Type u#a)) : Type u#a = DepMap.t field_id field_typs
+
+(** Helper function to prove that the recursive call of the next function is decreasing *)
+unfold
+let struct_field_type'
+      (field_descriptors: (field_id ^-> array_struct_descriptor u#a))
+      (array_struct_type:
+          (descriptor: array_struct_descriptor u#a {descriptor << field_descriptors}
+              -> Tot (Type u#a)))
+      (field: field_id)
+    : Tot (Type u#a) =
+  let descr = field_descriptors field in
+  FStar.WellFounded.axiom1 field_descriptors field;
+  array_struct_type descr
+
+(** This functions achives the [descriptor -> Type] correspondence *)
+let rec array_struct_type (descriptor: array_struct_descriptor u#a)
+    : Tot (Type u#a) (decreases descriptor) =
+  match descriptor with
+  | DBase a -> a
+  | DArray descriptor' len ->
+    let typ' = array_struct_type descriptor' in
+    array_type typ' len
+  | DStruct field_descriptors ->
+    let typs' = struct_field_type' field_descriptors array_struct_type in
+    struct_type typs'
+
+(** Gets the type of values of the field of a struct *)
+unfold
+let struct_field_type
+      (field_descriptors: (field_id ^-> (array_struct_descriptor u#a)))
+      (field: field_id)
+    : Tot (Type u#a) = struct_field_type' field_descriptors array_struct_type field
+
+(** The type of a struct value is a dependent map *)
+val struct_field_type_unroll_lemma (field_descriptors: (field_id ^-> array_struct_descriptor u#a))
+    : Lemma
+      (DependentMap.t u#a field_id (struct_field_type u#a field_descriptors) ==
+        array_struct_type u#a (DStruct u#a field_descriptors))
+      [SMTPat (array_struct_type u#a (DStruct u#a field_descriptors))]
+
+(**** The main [array_struct] type *)
+
+(**
+  [arraystruct] encapsulates the descriptor, a value corresponding to the descriptor as well as
+  a sub-PCM to govern the values corresponding to the descriptor. Note that the sub-PCM is unitless,
+  meaning that we don't require a unit value with its corresponding lemma. Indeed, the unit value
+  always comes from the [None] case of a base [option] type. We need a full-fledged PCM with a unit
+  value to store in the memory model, which is going to govern values of type [option array_struct].
+  But for the sub-PCM inside the [array_struct], we don't need a unit value.
+*)
+noeq
+type array_struct : Type u#(a + 1) =
+  | ArrayStruct : 
+      descriptor: array_struct_descriptor u#a ->
+      pcm: unitless_pcm (array_struct_type descriptor) ->
+      value: array_struct_type descriptor
+    -> array_struct
+
+/// Now, let's proceed to build the PCM that govern all arraystruct values stored inside the memory.
+
+(**
+  Composability is then based on the composability of the sub-PCM. Only arraystruct that have
+  the same descriptor and sub-PCM can be composed.
+*)
+let composable_array_struct:symrel u#(a + 1) (array_struct u#a) =
+  fun (s0: array_struct u#a) (s1: array_struct u#a) ->
+    s0.descriptor == s1.descriptor /\ s0.pcm == s1.pcm /\
+    s0.pcm.unitless_p.unitless_composable s0.value s1.value
+
+(** The composition also uses the sub-PCM's composition *)
+let compose_array_struct
+      (s0: array_struct u#a)
+      (s1: array_struct u#a {s0 `composable_array_struct` s1})
+    : array_struct u#a =
+  let new_val = s0.pcm.unitless_p.unitless_op s0.value s1.value in
+  ArrayStruct s0.descriptor s0.pcm new_val
+
+(** We can now define the unitless PCM for all [arraystruct] *)
+let array_struct_unitless_pcm:unitless_pcm u#(a + 1) (array_struct u#a) =
+  {
+    unitless_p
+    =
+    { unitless_composable = composable_array_struct u#a; unitless_op = compose_array_struct u#a };
+    unitless_comm = (fun s0 s1 -> s0.pcm.unitless_comm s0.value s1.value);
+    unitless_assoc = (fun s0 s1 s2 -> s0.pcm.unitless_assoc s0.value s1.value s2.value);
+    unitless_assoc_r = (fun s0 s1 s2 -> s0.pcm.unitless_assoc_r s0.value s1.value s2.value)
+  }
+
+(** To get a full-fledged PCM, we just add the [None] case *)
+let array_struct_pcm:pcm u#(a + 1) (option u#(a + 1) (array_struct u#a)) =
+  to_full_pcm_with_unit array_struct_unitless_pcm
+
+(*** Building a sub-PCM *)
+
+(**** For an array *)
+
+(**
+  This retrieves the composability for an array cell, given a base PCM governing the cells of
+  the array.
+*)
+let composable_array_cell
+      (#cell_type: Type u#a)
+      (#len: SizeT.t)
+      (base_pcm: unitless_pcm cell_type)
+      (x y: array_type cell_type len)
+      (i: nat{i < SizeT.v len})
+    : prop =
+  let xi = Seq.index x i in
+  let yi = Seq.index y i in
+  base_pcm.unitless_p.unitless_composable xi yi
+
+(** Composability for an array is pointwise composability of its cells *)
+let composable_array (#cell_type: Type u#a) (#len: SizeT.t) (base_pcm: unitless_pcm cell_type)
+    : symrel (array_type cell_type len) =
+  fun x y -> forall (i: nat{i < SizeT.v len}). composable_array_cell base_pcm x y i
+
+(** Composition for an array is pointwise composition of its cells*)
+let compose_array
+      (#cell_type: Type u#a)
+      (#len: SizeT.t)
+      (base_pcm: unitless_pcm cell_type)
+      (x: array_type cell_type len)
+      (y: array_type cell_type len {composable_array base_pcm x y})
+    : array_type cell_type len =
+  Seq.init (SizeT.v len)
+    (fun i ->
+        let xi = Seq.index x i in
+        let yi = Seq.index y i in
+        base_pcm.unitless_p.unitless_op xi yi)
+
+(**
+  From those composability and compose predicates we can build a sub-PCM for an array given the
+  sub-PCM governing its cells.
+*)
+val pointwise_array_pcm (cell_type: Type u#a) (len: SizeT.t) (base_pcm: unitless_pcm cell_type)
+    : unitless_pcm (array_type cell_type len)
+
+val reveal_pointwise_array_pcm
+      (cell_type: Type u#a)
+      (len: SizeT.t)
+      (base_pcm: unitless_pcm cell_type)
+    : Lemma
+      (let pcm = pointwise_array_pcm cell_type len base_pcm in
+        pcm.unitless_p.unitless_composable == composable_array base_pcm /\
+        pcm.unitless_p.unitless_op == compose_array base_pcm)
+      [SMTPat (pointwise_array_pcm cell_type len base_pcm)]
+
+(**** For a struct *)
+
+(**
+  This retrieves the composability for a struct field, given a base PCM governing the fields of
+  the struct.
+*)
+let composable_struct_field
+      (#field_types: (field_id -> Type u#a))
+      (base_pcms: (field: field_id -> unitless_pcm (field_types field)))
+      (field: field_id)
+      (x y: struct_type field_types)
+    : prop =
+  let xf = DepMap.sel x field in
+  let yf = DepMap.sel y field in
+  (base_pcms field).unitless_p.unitless_composable xf yf
+
+(** Composability for a struct is pointwise composability of its fields *)
+let composable_struct
+      (#field_types: (field_id -> Type u#a))
+      (base_pcms: (field: field_id -> unitless_pcm (field_types field)))
+    : symrel (struct_type field_types) =
+  fun x y -> forall (field: field_id). composable_struct_field base_pcms field x y
+
+(** Composition for a struct is pointwise composition of its fields *)
+let compose_struct
+      (#field_types: (field_id -> Type u#a))
+      (base_pcms: (field: field_id -> unitless_pcm (field_types field)))
+      (x: struct_type field_types)
+      (y: struct_type field_types {composable_struct base_pcms x y})
+    : struct_type field_types =
+  DepMap.create (fun field ->
+        let xf = DepMap.sel x field in
+        let yf = DepMap.sel y field in
+        (base_pcms field).unitless_p.unitless_op xf yf)
+
+(**
+  From those composability and compose predicates we can build a sub-PCM for a struct given the
+  sub-PCMs governing its fields.
+*)
+val pointwise_struct_pcm
+      (field_types: (field_id -> Type u#a))
+      (base_pcms: (field: field_id -> unitless_pcm (field_types field)))
+    : unitless_pcm (struct_type field_types)
+
+val reveal_pointwise_struct_pcm
+      (field_types: (field_id -> Type u#a))
+      (base_pcms: (field: field_id -> unitless_pcm (field_types field)))
+    : Lemma
+      (let pcm = pointwise_struct_pcm field_types base_pcms in
+        pcm.unitless_p.unitless_composable == composable_struct base_pcms /\
+        pcm.unitless_p.unitless_op == compose_struct base_pcms)
+      [SMTPat (pointwise_struct_pcm field_types base_pcms)]
+
+(*** Examples *)
+
+open Steel.PCM.FractionalPermission
+open Steel.PCM.Unitless.Base
+
+let array_with_frac_perm_on_all_indexes (t: Type u#a) (len: SizeT.t) (v: t) : array_struct u#a =
+  ArrayStruct (DArray (DBase (with_perm u#a t)) len)
+    (pointwise_array_pcm (with_perm t) len frac_perm_pcm)
+    (Seq.init u#a (SizeT.v len) (fun _ -> { value = v; perm = perm_one }))
+
+let immutable_splittable_array (t: Type u#a) (len: SizeT.t) (v: t) : array_struct u#a =
+  ArrayStruct (DArray (DBase t) len)
+    (pointwise_array_pcm t len immutable_unitless_pcm)
+    (Seq.init u#a (SizeT.v len) (fun _ -> v))
+
+let two_fields_restricted_func
+      (#a: Type u#a)
+      (field1: string)
+      (field2: string{field2 <> field1})
+      (value1 value2 by_default: a)
+    : (field_id ^-> a) =
+  on _
+    (fun field -> if field = field1 then value1 else if field = field2 then value2 else by_default)
+
+#push-options "--fuel 2 --ifuel 2"
+let two_fields_dep_map
+      (a: (field_id -> Type u#a))
+      (field1: string)
+      (field2: string{field2 <> field1})
+      (value1: a field1)
+      (value2: a field2)
+      (by_default: (field: field_id{field <> field1 /\ field <> field2} -> a field))
+    : (DepMap.t field_id a) =
+  DepMap.create #field_id
+    #a
+    (fun field ->
+        if field = field1 then value1 else if field = field2 then value2 else by_default field)
+
+let point_2d:array_struct =
+  let field_descriptors = two_fields_restricted_func "x" "y" (DBase int) (DBase int) (DBase unit) in
+  let field_types:(field_id -> Type0) = struct_field_type field_descriptors in
+  let field_pcms:(field: field_id -> unitless_pcm (field_types field)) =
+    fun field ->
+      if field = "x"
+      then exclusive_unitless_pcm
+      else if field = "y" then immutable_unitless_pcm else exclusive_unitless_pcm
+  in
+  struct_field_type_unroll_lemma field_descriptors;
+  ArrayStruct (DStruct field_descriptors)
+    (pointwise_struct_pcm field_types field_pcms)
+    (two_fields_dep_map field_types "x" "y" 0 1 (fun _ -> ()))
+
